Splinter/Betree/BranchSeq.i.dfy
@@ -1,0 +1,85 @@
+// Copyright 2018-2021 VMware, Inc., Microsoft Inc., Carnegie Mellon University, ETH Zurich, and University of Washington
+// SPDX-License-Identifier: BSD-2-Clause
+
+include "../Disk/GenericDisk.i.dfy"
+include "LinkedBranch.i.dfy"
+
+module BranchSeqMod {
+  import opened KeyType
+  import opened ValueMessage
+  import opened Maps
+  import opened Sequences
+  import opened OffsetMapMod
+  import opened LinkedBranchMod
+  import D = GenericDisk
+
+  // track a sequence of roots
+  datatype BranchSeq = BranchSeq(roots: seq<Address>)
+  {
+    // predicate Valid(dv: DiskView)
+    // {
+    //   && (forall i:nat | i < |roots| :: roots[i] in dv.Representation())
+    //   && (forall i:nat | i < |roots| :: LinkedBranch(roots[i], dv).Acyclic())
+    // }
+
+    function Length() : nat 
+    {
+      |roots|
+    }
+
+    function Representation() : set<Address>
+    {
+      set addr | addr in roots
+    }
+
+    function Slice(start: nat, end: nat) : BranchSeq
+      requires start <= end <= |roots|
+    {
+      BranchSeq(roots[start..end])
+    }
+
+    function Extend(newBranchSeq: BranchSeq) : BranchSeq
+    {
+      BranchSeq(roots + newBranchSeq.roots)
+    }
+
+    function QueryFrom(dv: DiskView, key: Key, start: nat) : Message
+      requires start <= |roots|
+      decreases |roots| - start
+    {
+      if start == |roots| then Update(NopDelta())
+      else (
+        var branch := LinkedBranch(roots[start], dv);
+        var msg := if branch.Acyclic() then branch.Query(key) else Update(NopDelta());
+        Merge(QueryFrom(dv, key, start+1), msg)
+      )
+    }
+
+    function DropFirst() : BranchSeq
+      requires 0 < |roots|
+    {
+      Slice(1, |roots|)
+    }
+
+    function QueryFiltered(dv: DiskView, offsetMap: OffsetMap, key: Key) : Message
+      requires offsetMap.WF()
+      decreases Length()
+    {
+      if |roots| == 0 then Update(NopDelta())
+      else (
+        var branch := LinkedBranch(roots[0], dv);
+        var msg := 
+          if branch.Acyclic() && key in offsetMap.FilterForBottom() 
+          then branch.Query(key) else Update(NopDelta());
+        Merge(DropFirst().QueryFiltered(dv, offsetMap.Decrement(1), key), msg)
+      )
+    }
+
+    predicate QueryFilteredEquiv(dv: DiskView, offsetMap: OffsetMap, newBranch: LinkedBranch)
+      requires offsetMap.WF()
+      requires newBranch.Acyclic()
+    {
+      && (forall key :: QueryFiltered(dv, offsetMap, key) == newBranch.Query(key))    
+    }
+  }  // end type BranchSeq
+}
